FOL/Program/LN/Binders.lean
@@ -1,0 +1,137 @@
+import FOL.Program.LN.Formula
+import FOL.Tactics
+
+
+namespace LN
+
+open Formula
+
+
+/--
+  Var.isFree v := True if and only if v is a free variable.
+-/
+def Var.isFree : Var → Prop
+  | free_ _ => True
+  | bound_ _ => False
+
+instance (v : Var) : Decidable v.isFree :=
+  by
+  cases v
+  case free_ x =>
+    simp only [Var.isFree]
+    exact decidableTrue
+  case bound_ i =>
+    simp only [Var.isFree]
+    exact decidableFalse
+
+
+/--
+  Var.isBound v := True if and only if v is a bound variable.
+-/
+def Var.isBound : Var → Prop
+  | free_ _ => False
+  | bound_ _ => True
+
+instance (v : Var) : Decidable v.isBound :=
+  by
+  cases v
+  case free_ x =>
+    simp only [Var.isBound]
+    exact decidableFalse
+  case bound_ i =>
+    simp only [Var.isBound]
+    exact decidableTrue
+
+--------------------------------------------------
+
+/--
+  Formula.var F := The set of all of the variables that have an occurrence in the formula F.
+-/
+def Formula.varSet : Formula → Finset Var
+  | pred_ _ vs => vs.toFinset
+  | not_ phi => phi.varSet
+  | imp_ phi psi => phi.varSet ∪ psi.varSet
+  | forall_ _ phi => phi.varSet
+
+
+/--
+  occursIn v F := True if and only if there is an occurrence of the variable v in the formula F.
+-/
+def occursIn (v : Var) : Formula → Prop
+  | pred_ _ vs => v ∈ vs
+  | not_ phi => occursIn v phi
+  | imp_ phi psi => occursIn v phi ∨ occursIn v psi
+  | forall_ _ phi => occursIn v phi
+
+
+instance (v : Var) (F : Formula) : Decidable (occursIn v F) :=
+  by
+  induction F
+  all_goals
+    unfold occursIn
+    infer_instance
+
+--------------------------------------------------
+
+/--
+  Formula.freeVarSet F := The set of all of the free variables that have an occurrence in the formula F.
+-/
+def Formula.freeVarSet (F : Formula) : Finset Var :=
+  F.varSet.filter Var.isFree
+
+/--
+  Formula.boundVarSet F := The set of all of the bound variables that have an occurrence in the formula F.
+-/
+def Formula.boundVarSet (F : Formula) : Finset Var :=
+  F.varSet.filter Var.isBound
+
+--------------------------------------------------
+
+theorem occursIn_iff_mem_varSet
+  (v : Var)
+  (F : Formula) :
+  occursIn v F ↔ v ∈ F.varSet :=
+  by
+  induction F
+  case pred_ X vs =>
+    simp only [occursIn]
+    simp only [varSet]
+    simp
+  case not_ phi phi_ih =>
+    simp only [occursIn]
+    simp only [varSet]
+    exact phi_ih
+  case imp_ phi psi phi_ih psi_ih =>
+    simp only [occursIn]
+    simp only [varSet]
+    simp
+    congr!
+  case forall_ _ phi phi_ih =>
+    simp only [occursIn]
+    simp only [varSet]
+    exact phi_ih
+
+
+theorem isFreeIn_iff_mem_freeVarSet
+  (v : Var)
+  (F : Formula) :
+  occursIn v F ∧ v.isFree ↔ v ∈ F.freeVarSet :=
+  by
+  simp only [freeVarSet]
+  simp
+  intro _
+  exact occursIn_iff_mem_varSet v F
+
+
+theorem isBoundIn_iff_mem_boundVarSet
+  (v : Var)
+  (F : Formula) :
+  occursIn v F ∧ v.isBound ↔ v ∈ F.boundVarSet :=
+  by
+  simp only [boundVarSet]
+  simp
+  intro _
+  exact occursIn_iff_mem_varSet v F
+
+
+#lint
